Lemmas/List/Instances.lean
@@ -13,7 +13,7 @@ public import Std.Tactic.Do.Syntax
 
 public import Lemmas.Lemmas
 
-open Lean Lean.Syntax Parser Parser.Char
+open Lean Lean.Syntax Parser
 
 open Std.Do
 
@@ -39,18 +39,18 @@ instance : Parser.Stream.AllValid (Parser.Stream.OfList τ) where
 @[simp] def respectsPosition (it rem : (Parser.Stream.OfList τ)) :=
   it.past.reverse ++ it.next = rem.past.reverse ++ rem.next
 
-@[simp] private theorem fwdZeroEq (it : (Stream.OfList τ))
+@[simp] private theorem fwd_zero_eq (it : (Stream.OfList τ))
     : (Stream.OfList.setPosition.fwd 0 it) = it := by
   simp [Stream.OfList.setPosition.fwd]
 
-@[simp] private theorem fwdIncrEq (n : Nat)
+@[simp] private theorem fwd_incr_eq (n : Nat)
     : (Stream.OfList.setPosition.fwd (n + 1) ⟨x :: next, past⟩)
       = (Stream.OfList.setPosition.fwd n ⟨next, x :: past⟩) := by
   generalize heq : Stream.OfList.setPosition.fwd n ⟨next, x :: past⟩ = f
   unfold Stream.OfList.setPosition.fwd
   simp_all
 
-private theorem fwdTakeReverseEq (it : (Parser.Stream.OfList τ)) (n) (h : n ≤ it.next.length)
+private theorem fwd_take_reverse_eq (it : (Parser.Stream.OfList τ)) (n) (h : n ≤ it.next.length)
     : Stream.OfList.setPosition.fwd n ⟨it.next, it.past⟩
       = ⟨it.next.drop n, (it.next.take n).reverse ++ it.past⟩ := by
   induction n generalizing it
@@ -62,23 +62,23 @@ private theorem fwdTakeReverseEq (it : (Parser.Stream.OfList τ)) (n) (h : n ≤
       simp [*]
     | [] => simp_all
 
-private theorem fwdPastLengthEq (it : (Parser.Stream.OfList τ)) (n : Nat) (hle : n ≤ it.next.length)
+private theorem fwd_past_length_eq (it : (Parser.Stream.OfList τ)) (n : Nat) (hle : n ≤ it.next.length)
     : (Stream.OfList.setPosition.fwd n it).past.length = it.past.length + n := by
-  rw [fwdTakeReverseEq it n hle]
+  rw [fwd_take_reverse_eq it n hle]
   simp_all +arith
 
-@[simp] private theorem revZeroEq (it : (Stream.OfList τ))
+@[simp] private theorem rev_zero_eq (it : (Stream.OfList τ))
     : (Stream.OfList.setPosition.rev 0 it) = it := by
   simp [Stream.OfList.setPosition.rev]
 
-@[simp] private theorem revIncrEq (n : Nat)
+@[simp] private theorem rev_incr_eq (n : Nat)
     : (Stream.OfList.setPosition.rev (n + 1) ⟨next, x :: past⟩)
       = (Stream.OfList.setPosition.rev n ⟨x :: next, past⟩) := by
   generalize heq : Stream.OfList.setPosition.rev n ⟨x :: next, past⟩ = f
   unfold Stream.OfList.setPosition.rev
   simp_all
 
-private theorem revTakeReverseEq (it : (Parser.Stream.OfList τ)) (n) (h : n ≤ it.past.length)
+private theorem rev_take_reverse_eq (it : (Parser.Stream.OfList τ)) (n) (h : n ≤ it.past.length)
     : Stream.OfList.setPosition.rev n ⟨it.next, it.past⟩
       = ⟨(it.past.take n).reverse ++ it.next, it.past.drop n⟩ := by
   induction n generalizing it
@@ -90,13 +90,13 @@ private theorem revTakeReverseEq (it : (Parser.Stream.OfList τ)) (n) (h : n ≤
       simp [*]
     | [] => simp_all
 
-private theorem revPastLengthEq (it : (Parser.Stream.OfList τ)) (n : Nat) (hle : n ≤ it.past.length)
+private theorem rev_past_length_eq (it : (Parser.Stream.OfList τ)) (n : Nat) (hle : n ≤ it.past.length)
     : (Stream.OfList.setPosition.rev n it).past.length = it.past.length - n := by
-  rw [revTakeReverseEq it n hle]
+  rw [rev_take_reverse_eq it n hle]
   simp_all +arith
 
 /-- Stream.SetPositionPrecondition -/
-theorem setPositionPrecondition (it : (Parser.Stream.OfList τ))
+theorem setPosition_precondition (it : (Parser.Stream.OfList τ))
   (pos : Stream.Position (Parser.Stream.OfList τ))
     : pos ≤ it.past.length + it.next.length
       → ∃ rem, Stream.setPosition it pos = rem
@@ -106,15 +106,15 @@ theorem setPositionPrecondition (it : (Parser.Stream.OfList τ))
   intro h
   and_intros
   · split
-    · rw [fwdPastLengthEq it (pos - it.past.length) (Nat.sub_le_iff_le_add'.mpr h)]
+    · rw [fwd_past_length_eq it (pos - it.past.length) (Nat.sub_le_iff_le_add'.mpr h)]
       grind
-    · rw [revPastLengthEq it (it.past.length - pos) (Nat.sub_le it.past.length pos)]
+    · rw [rev_past_length_eq it (it.past.length - pos) (Nat.sub_le it.past.length pos)]
       grind
   · split
-    · have := fwdTakeReverseEq it (pos - it.past.length) (Nat.sub_le_iff_le_add'.mpr h)
+    · have := fwd_take_reverse_eq it (pos - it.past.length) (Nat.sub_le_iff_le_add'.mpr h)
       rw [this]
       simp
-    · have := revTakeReverseEq it (it.past.length - pos) (Nat.sub_le it.past.length pos)
+    · have := rev_take_reverse_eq it (it.past.length - pos) (Nat.sub_le it.past.length pos)
       rw [this]
       rw [← List.append_assoc, ← List.reverse_append]
       simp_all
@@ -123,7 +123,7 @@ theorem setPositionPrecondition (it : (Parser.Stream.OfList τ))
 theorem setPositionOfGetPositionEqIfRespectsPosition (s1 s2 : (Parser.Stream.OfList τ))
   (p) (h1 : Stream.getPosition s1 = p) (h2 : respectsPosition s1 s2)
     : Stream.setPosition s2 p = s1 := by
-  have ⟨r, And.intro hr ⟨hg, hs⟩ ⟩ := setPositionPrecondition s2 p (by
+  have ⟨r, And.intro hr ⟨hg, hs⟩ ⟩ := setPosition_precondition s2 p (by
     simp [Stream.getPosition] at h1
     simp [respectsPosition] at h2
     have : (s2.past.reverse ++ s2.next).length = (s1.past.reverse ++ s1.next).length := by grind      --have : s2.past.length + s2.next.length = s1.past.length + s1.next.length := by grind
@@ -144,17 +144,16 @@ theorem setPositionOfGetPositionEqIfRespectsPosition (s1 s2 : (Parser.Stream.OfL
   grind
 
 instance : Stream.RespectsPosition (Parser.Stream.OfList τ) τ where
-  respectsPosition := respectsPosition
-  setPositionOfGetPositionEq s1 s2 p :=
+  r := respectsPosition
+  setPosition_of_getPosition_eq s1 s2 p :=
     fun h => setPositionOfGetPositionEqIfRespectsPosition s1 s2 p
   isEquivalence := Equivalence.mk (by simp) (by simp; grind) (by simp; grind)
 
 instance : Stream.SetPositionPrecondition (Parser.Stream.OfList τ) τ where
   cond it pos := pos ≤ it.past.length + it.next.length
-  validResult it pos := setPositionPrecondition it pos
-  ofGetPosition (s1 s2 : Parser.Stream.OfList τ) (p : Stream.Position (Parser.Stream.OfList τ)) := by
-    simp [Stream.ValidPosition.valid, Stream.RespectsPosition.respectsPosition,
-          Stream.getPosition]
+  valid it pos := setPosition_precondition it pos
+  of_getPosition (s1 s2 : Parser.Stream.OfList τ) (p : Stream.Position (Parser.Stream.OfList τ)) := by
+    simp [Stream.ValidPosition.valid, Stream.respectsPosition, Stream.RespectsPosition.r, Stream.getPosition]
     intro h1 h2
     rw [← h1]
     have : (s2.past.reverse ++ s2.next).length = (s1.past.reverse ++ s1.next).length := by grind
@@ -162,7 +161,7 @@ instance : Stream.SetPositionPrecondition (Parser.Stream.OfList τ) τ where
     rw [this]
     simp
 
-private theorem next?SomeOfLt (it : Parser.Stream.OfList τ)
+private theorem next?_some (it : Parser.Stream.OfList τ)
   (h : 0 < Stream.Remaining.remaining it)
     : ∃ rem c, Std.Stream.next? it = some (c, rem) ∧ Stream.decrementsRemaining it rem
                                   ∧ respectsPosition it rem := by
@@ -174,13 +173,13 @@ private theorem next?SomeOfLt (it : Parser.Stream.OfList τ)
   split <;> simp_all
 
 instance : Stream.Next?OnInput (Parser.Stream.OfList τ) τ where
-  cond := next?SomeOfLt
+  cond := next?_some
 
-private theorem next?None (it : Parser.Stream.OfList τ) (h : 0 = Stream.Remaining.remaining it)
+private theorem next?_none (it : Parser.Stream.OfList τ) (h : 0 = Stream.Remaining.remaining it)
     : Std.Stream.next? it = none := by
   simp [Stream.Remaining.remaining] at h
   simp [Std.Stream.next?]
   split <;> simp_all
 
 instance : Stream.Next?OnEndOfInput (Parser.Stream.OfList τ) τ where
-  cond it _ h := next?None it h
+  cond it _ h := next?_none it h
