Lemmas/SimpLemmas.lean
@@ -1,0 +1,78 @@
+module
+
+public import Init.Meta
+
+import all Parser.Basic
+import all Parser.Error
+import all Parser.Parser
+import all Parser.Prelude
+import all Parser.Stream
+
+public import Std.Tactic.Do
+public import Std.Tactic.Do.Syntax
+
+public import Lemmas.Basic
+public import Lemmas.Instances
+
+open Lean Lean.Syntax Parser
+
+open Std.Do
+
+@[expose] public section
+
+namespace Parser
+
+/-! Simp lemmas for SimpleParser σ τ -/
+
+@[grind .] theorem SimpleParser.getPosition_eq_ok [Parser.Stream σ τ] (it : σ)
+    : (getPosition : SimpleParser σ τ _) it = Result.ok it (Stream.getPosition it) := by
+  simp [getPosition, Functor.map]
+  rfl
+
+@[simp] theorem setPosition_eq_ok  [Parser.Stream σ τ] (s1 : σ) (p : Stream.Position σ)
+    : ∃ (s2 : σ), (setPosition p : SimpleParser σ τ Unit) s1 = Result.ok s2 () :=
+  Exists.intro (Stream.setPosition s1 p) rfl
+
+@[simp] theorem SimpleParser.throw_eq_error [Parser.Stream σ τ] (it : σ) (e : Error.Simple σ τ)
+    : (MonadExcept.throw e : SimpleParser σ τ α) it = Result.error it e := by
+  simp [throw, throwThe, MonadExceptOf.throw, pure]
+
+@[simp, grind .] theorem throwUnexpected_eq_error [Parser.Stream σ τ]
+    (α : Type) (s : σ) (c : Option τ)
+    : (throwUnexpected c s : Id (Parser.Result (Error.Simple σ τ) σ α))
+      = Result.error s (Error.unexpected (Stream.getPosition s) c) := by
+  simp only [throwUnexpected, bind, throw, throwThe, MonadExceptOf.throw, pure]
+  rfl
+
+@[simp] theorem SimpleParser.WP.seqRight (σ τ : Type) [Parser.Stream σ τ] [Stream.Remaining σ]
+  [Stream.ValidPosition σ] [Stream.RespectsPosition σ τ]
+  (p : SimpleParser σ τ α) (q : SimpleParser σ τ β)
+  {Q : PostCond β (.except (Error.Simple σ τ) (.arg σ .pure))}
+    : wp⟦p *> q⟧ Q = wp⟦p⟧ (fun _ => wp⟦q⟧ Q, Q.2) := by
+  simp [wp, SeqRight.seqRight, PredTrans.apply, Parser.run, bind, pure]
+  funext
+  grind
+
+@[simp] theorem SimpleParser.WP.tryCatch (σ τ : Type) [Parser.Stream σ τ] [Stream.Remaining σ]
+  [Stream.ValidPosition σ] [Stream.RespectsPosition σ τ]
+  (p : SimpleParser σ τ α) (h : (Error.Simple σ τ) → SimpleParser σ τ α)
+  {Q : PostCond α (.except (Error.Simple σ τ) (.arg σ .pure))}
+    : wp⟦MonadExceptOf.tryCatch p h⟧ Q
+      = wp⟦p⟧ (Q.1, fun e => wp⟦h e⟧ Q, Q.snd.snd) := by
+  simp [wp, MonadExceptOf.tryCatch, PredTrans.apply, pure, bind, ParserT.run, Parser.run]
+  funext
+  grind
+
+@[simp] theorem SimpleParser.WP.throwErrorWithMessage (σ τ : Type) [Parser.Stream σ τ] [Stream.Remaining σ]
+  [Stream.ValidPosition σ] [Stream.RespectsPosition σ τ]
+  (e : Error.Simple σ τ) (msg : String)
+  {Q : PostCond α (.except (Error.Simple σ τ) (.arg σ .pure))}
+    : wp⟦(throwErrorWithMessage e msg : SimpleParser σ τ α)⟧ Q
+      = fun s => Q.2.1 (Error.addMessage e (Stream.getPosition s) msg) s := by
+  simp [wp, PredTrans.apply, Parser.throwErrorWithMessage, Parser.run, bind, pure]
+  funext
+  split
+  · rename_i heq
+    split at heq <;> simp_all
+  · rename_i heq
+    grind
