Lemmas/String/Instances.lean
@@ -14,7 +14,7 @@ import Std.Tactic.Do.Syntax
 public import Lemmas.Lemmas
 public import Lemmas.String.Basic
 
-open Lean Lean.Syntax Parser Parser.Char
+open Lean Lean.Syntax Parser
 
 open Std.Do
 
@@ -40,7 +40,7 @@ instance : Parser.Stream.AllValid String.Slice where
 @[simp] def respectsPosition (it rem : String.Slice) :=
   it.str = rem.str ∧ it.endExclusive.offset = rem.endExclusive.offset
 
-private theorem slice!PosEq (s : String) (p₁ p₂ : s.Pos) (h : p₁.offset ≤ p₂.offset)
+private theorem slice!_eq (s : String) (p₁ p₂ : s.Pos) (h : p₁.offset ≤ p₂.offset)
     : (String.slice! s p₁ p₂).startInclusive.offset = p₁.offset
       ∧ (String.slice! s p₁ p₂).endExclusive.offset = p₂.offset
       ∧ (String.slice! s p₁ p₂).str = s := by
@@ -48,14 +48,14 @@ private theorem slice!PosEq (s : String) (p₁ p₂ : s.Pos) (h : p₁.offset �
   simp
 
 /-- Stream.SetPositionPrecondition -/
-theorem setPositionPrecondition (it : String.Slice) (pos : Stream.Position String.Slice)
+theorem setPosition_precondition (it : String.Slice) (pos : Stream.Position String.Slice)
   : pos.IsValid it.str ∧ pos ≤ it.endExclusive.offset
     → ∃ rem, Stream.setPosition it pos = rem
               ∧ pos = Parser.Stream.getPosition rem
               ∧ respectsPosition it rem := by
   simp [Stream.setPosition, Stream.getPosition]
   intro h1 h2
-  have := slice!PosEq it.str ⟨pos, by grind⟩ ⟨it.endExclusive.offset, it.endExclusive.isValid⟩
+  have := slice!_eq it.str ⟨pos, by grind⟩ ⟨it.endExclusive.offset, it.endExclusive.isValid⟩
             (by simp_all)
   generalize hg : (if h : String.Pos.Raw.IsValid it.str pos
       then it.str.slice! { offset := pos, isValid := by grind } it.endExclusive
@@ -75,7 +75,7 @@ theorem setPositionPrecondition (it : String.Slice) (pos : Stream.Position Strin
     · simp_all
 
 /-- no input is consumed if the position is reset after applying a respectful parser -/
-theorem setPositionOfGetPositionEqIfRespectsPosition (s1 s2 : String.Slice) (p)
+theorem setPosition_of_getPosition_eq (s1 s2 : String.Slice) (p)
   (h1 : Stream.getPosition s1 = p) (h2 : respectsPosition s1 s2)
     : Stream.setPosition s2 p = s1 := by
   simp [Stream.getPosition] at h1
@@ -85,25 +85,25 @@ theorem setPositionOfGetPositionEqIfRespectsPosition (s1 s2 : String.Slice) (p)
     rw [← h1, ← h2.left]
     exact s1.startInclusive.isValid
   split
-  · have := slice!PosEq s2.str ⟨p, by grind⟩ ⟨s2.endExclusive.offset, s2.endExclusive.isValid⟩
+  · have := slice!_eq s2.str ⟨p, by grind⟩ ⟨s2.endExclusive.offset, s2.endExclusive.isValid⟩
             (by simp; rw [← h2.right, ← h1]; exact s1.startInclusive_le_endExclusive)
     exact @String.Slice.ext (s2.str.slice! { offset := p, isValid := by grind } s2.endExclusive) s1
             (by simp_all) (by simp_all) (by simp_all)
   · simp_all
 
 instance : Stream.RespectsPosition String.Slice Char where
-  respectsPosition := respectsPosition
-  setPositionOfGetPositionEq s1 s2 p :=
-    fun h => setPositionOfGetPositionEqIfRespectsPosition s1 s2 p
+  r := respectsPosition
+  setPosition_of_getPosition_eq s1 s2 p :=
+    fun h => setPosition_of_getPosition_eq s1 s2 p
   isEquivalence := Equivalence.mk (by simp) (by simp; grind) (by simp; grind)
 
 instance : Stream.SetPositionPrecondition String.Slice Char where
   cond it pos := pos.IsValid it.str ∧ pos ≤ it.endExclusive.offset
-  validResult it pos := setPositionPrecondition it pos
-  ofGetPosition (s1 s2 : String.Slice) (p : Stream.Position String.Slice) := by
+  valid it pos := setPosition_precondition it pos
+  of_getPosition (s1 s2 : String.Slice) (p : Stream.Position String.Slice) := by
     intro _ h1 h2
     simp [Stream.getPosition] at h1
-    simp [Stream.RespectsPosition.respectsPosition] at h2
+    simp [Stream.respectsPosition] at h2
     and_intros
     · rw [← h1, ← h2.left]
       exact s1.startInclusive.isValid
@@ -112,11 +112,11 @@ instance : Stream.SetPositionPrecondition String.Slice Char where
         exact s1.startInclusive_le_endExclusive
       simp_all
 
-@[simp, grind .] private theorem eqOfRemaining (it : String.Slice)
+@[simp, grind .] private theorem eq_of_remaining (it : String.Slice)
     : Stream.Remaining.remaining it =  it.endExclusive.offset.byteIdx - it.startInclusive.offset.byteIdx := by
   simp [Stream.Remaining.remaining, String.Slice.utf8ByteSize, String.Pos.Raw.byteDistance]
 
-@[grind .] private theorem ltOfRemaining_iff (it : String.Slice)
+@[grind .] private theorem lt_of_remaining_iff (it : String.Slice)
     :  0 < Stream.Remaining.remaining it ↔ it.startInclusive.offset < it.endExclusive.offset := by
   simp [Stream.Remaining.remaining, String.Slice.utf8ByteSize, String.Pos.Raw.byteDistance]
   exact Iff.intro
@@ -135,7 +135,7 @@ instance : Stream.SetPositionPrecondition String.Slice Char where
       exact String.Pos.Raw.ext this)
     (fun h => by simp_all)
 
-private theorem startPosNeEndPosOfLt (it : String.Slice)
+private theorem startPos_ne_endPos_of_lt (it : String.Slice)
   (h : it.startInclusive.offset < it.endExclusive.offset)
     : it.startPos != it.endPos := by
   simp [String.Slice.startPos, String.Slice.endPos]
@@ -144,7 +144,7 @@ private theorem startPosNeEndPosOfLt (it : String.Slice)
     assumption
   grind
 
-private theorem startPosEqEndPosOfEq (it : String.Slice)
+private theorem startPos_eq_endPos_of_eq (it : String.Slice)
   (h : it.startInclusive.offset = it.endExclusive.offset)
     : it.startPos = it.endPos := by
   simp [String.Slice.startPos, String.Slice.endPos]
@@ -153,24 +153,24 @@ private theorem startPosEqEndPosOfEq (it : String.Slice)
     simp_all
   grind
 
-private theorem sliceOfNextLt (it : String.Slice) (h : it.startPos ≠ it.endPos)
+private theorem offset_lt_of_pos_ne (it : String.Slice) (h : it.startPos ≠ it.endPos)
     : it.startInclusive.offset.byteIdx < (it.startPos.next h).str.offset.byteIdx := by
   simp [String.Slice.Pos.get, String.decodeChar, Char.utf8Size]
   grind
 
-private theorem next?SomeOfLt (it : String.Slice)
+private theorem next?_some (it : String.Slice)
   (h : 0 < Stream.Remaining.remaining it)
     : ∃ rem c, Std.Stream.next? it = some (c, rem) ∧ Stream.decrementsRemaining it rem
                                   ∧ respectsPosition it rem := by
   simp [Std.Stream.next?, String.Slice.front?, String.Slice.Pos.get?, bind, Option.bind]
-  have := startPosNeEndPosOfLt it (by grind)
+  have := startPos_ne_endPos_of_lt it (by grind)
   simp at this
   split
   · grind
   · expose_names
     split at heq
     · grind
-    · have := String.Pos.Raw.lt_iff.mpr (sliceOfNextLt it (by grind))
+    · have := String.Pos.Raw.lt_iff.mpr (offset_lt_of_pos_ne it (by grind))
       simp_all [Stream.decrementsRemaining]
       have := Char.utf8Size_pos a
       simp_all
@@ -179,17 +179,17 @@ private theorem next?SomeOfLt (it : String.Slice)
       grind
 
 instance : Stream.Next?OnInput String.Slice Char where
-  cond := next?SomeOfLt
+  cond := next?_some
 
-private theorem next?None (it : String.Slice) (h : 0 = Stream.Remaining.remaining it)
+private theorem next?_none (it : String.Slice) (h : 0 = Stream.Remaining.remaining it)
     : Std.Stream.next? it = none := by
   simp [Std.Stream.next?, String.Slice.front?, String.Slice.Pos.get?,
         bind, Option.bind]
   split
   · rfl
   · rename_i heq
-    have := startPosEqEndPosOfEq it ((eqOfRemaining_iff it).mp h)
+    have := startPos_eq_endPos_of_eq it ((eqOfRemaining_iff it).mp h)
     split at heq <;> simp_all
 
 instance : Stream.Next?OnEndOfInput String.Slice Char where
-  cond it _ h := next?None it h
+  cond it _ h := next?_none it h
